Eqsat/EGraph/Basic.lean
@@ -1,0 +1,21 @@
+import Eqsat.TreeAutomaton.Reachable
+import Eqsat.PCR
+
+/- **Definition 3** -/
+structure EGraph (S Q) [Signature S] extends auto : TreeAutomaton S Q where
+  det      : auto.Deterministic
+  reach    : auto.Reachable
+  no_final : auto.final = ∅
+
+namespace EGraph
+
+variable [Signature S] {graph : EGraph S Q}
+
+abbrev EClass (_ : EGraph S Q) := Q
+
+abbrev ENode (_ : EGraph S Q) := TreeAutomaton.Transition S Q
+
+abbrev EClass.Represents (c : EClass graph) (t : Term S) : Prop :=
+  graph.Accepts c t
+
+end EGraph
