Eqsat/EGraph/PCR.lean
@@ -1,0 +1,102 @@
+import Eqsat.EGraph.Basic
+
+variable [Signature S]
+
+/- **Definition 5** -/
+def EGraph.pcr (graph : EGraph S Q) : PCR S where
+  rel t₁ t₂ :=
+    ∃ c : EClass graph, c.Represents t₁ ∧ c.Represents t₂
+  symm := by
+    grind [Symmetric]
+  trans _ _ _ := by
+    simp only [forall_exists_index, and_imp]
+    intro c _ h₁ _ h₂ _
+    exists c
+    have := graph.det h₁ h₂
+    simp_all
+  congr h mem := open TreeAutomaton TRS.Steps in by
+    rename_i fn as bs
+    simp only [PER.support, and_self] at mem
+    obtain ⟨c, hc⟩ := mem
+    refine ⟨c, hc, ?_⟩
+    have ⟨qs, hq₁, hq₂⟩ := hc.final
+    apply tail (children fun i => ?_) (step_of_transition hq₁)
+    have ⟨_, hc₁, hc₂⟩ := h i
+    obtain ⟨rfl⟩ := graph.det hc₁ <| steps_child hq₂ i
+    exact hc₂
+  reach h i := by
+    simp only [PER.support, and_self, Set.mem_setOf_eq] at *
+    obtain ⟨_, h⟩ := h
+    apply h.child
+
+/- **Theorem 6** -/
+namespace PCR
+
+variable {graph : EGraph S Q}
+
+inductive IsAutomatonTransition (pcr : PCR S) : (TreeAutomaton.Transition S pcr.Classes) → Prop
+  | intro (mem₁ : fn ° as ∈ pcr.support) (mem₂ : ∀ i, as i ∈ pcr.support) :
+    IsAutomatonTransition pcr ⟨fn, fun i => ⟦⟨as i, mem₂ i⟩⟧, ⟦⟨fn ° as, mem₁⟩⟧⟩
+
+def automaton (pcr : PCR S) : TreeAutomaton S pcr.Classes where
+  trans := { tr | pcr.IsAutomatonTransition tr }
+  final := ∅
+
+open TreeAutomaton Signature.Extended in section
+
+theorem automaton_step_deterministic {pcr : PCR S} {t : Term _} {q₁ q₂ : pcr.Classes}
+    (h₁ : t -[pcr.automaton]→ q₁) (h₂ : t -[pcr.automaton]→ q₂) : q₁ = q₂ := by
+  let fn ° as := t
+  obtain ⟨_, ⟨mem₁₁, mem₁₂⟩, h₁⟩ := mem_trs_to_trans h₁.rw_of_ext.choose_spec
+  obtain ⟨_, ⟨mem₂₁, mem₂₂⟩, h₂⟩ := mem_trs_to_trans h₂.rw_of_ext.choose_spec
+  simp only [Transition.toRewrite, Rewrite.mk.injEq, Pattern.app.injEq, ext.injEq] at h₁ h₂
+  obtain ⟨⟨rfl, rfl⟩, rfl, _⟩ := h₁
+  obtain ⟨⟨⟨rfl, rfl⟩, h⟩, rfl, _⟩ := h₂
+  rename_i fn as₁ _ as₂ _
+  have h i : (⟦⟨as₁ i, mem₁₂ _⟩⟧ : Quotient pcr.supportSetoid) = ⟦⟨as₂ i, mem₂₂ _⟩⟧ := by
+    have := congrFun (eq_of_heq h) i
+    simp_all
+  exact Quotient.sound <| @pcr.congr fn as₁ as₂ (Quotient.eq.mp <| h ·) mem₁₁
+
+theorem automaton_deterministic (pcr : PCR S) : pcr.automaton.Deterministic := by
+  intro t q₁ q₂ hq₁ hq₂
+  let fn ° as := t
+  have ⟨qs₁, mem₁, h₁⟩ := hq₁.final
+  have ⟨qs₂, mem₂, h₂⟩ := hq₂.final
+  have h := funext fun i => automaton_deterministic pcr (steps_child h₁ i) (steps_child h₂ i)
+  exact automaton_step_deterministic (step_of_transition mem₁) (step_of_transition <| h ▸ mem₂)
+
+theorem automaton_reachable (pcr : PCR S) : pcr.automaton.Reachable := by
+  refine Quotient.ind fun ⟨t, h⟩ => ⟨t, ?_⟩
+  induction t
+  case app ih =>
+    exact .tail (.children fun i => ih i <| pcr.reach h i) (step_of_transition <| .intro ..)
+
+end
+
+def egraph (pcr : PCR S) : EGraph S pcr.Classes where
+  auto     := pcr.automaton
+  no_final := rfl
+  det      := pcr.automaton_deterministic
+  reach    := pcr.automaton_reachable
+
+open EGraph
+
+theorem egraph_correct (pcr : PCR S) : pcr.egraph.pcr = pcr := by
+  ext t₁ t₂
+  have acc₁ : pcr.egraph.Accepts ⟦⟨t₁, sorry⟩⟧ t₁ := sorry
+  have acc₂ : pcr.egraph.Accepts ⟦⟨t₂, sorry⟩⟧ t₂ := sorry
+  apply Iff.intro (fun h => ?mp) (fun h => ?mpr)
+  case mp =>
+    obtain ⟨c, hc₁, hc₂⟩ := h
+    exact Quotient.eq.mp <| pcr.egraph.det acc₂ hc₂ ▸ pcr.egraph.det acc₁ hc₁
+  case mpr h =>
+    replace h : (⟦⟨t₁, sorry⟩⟧ : pcr.Classes) = ⟦⟨t₂, sorry⟩⟧ := sorry
+    exact ⟨_, acc₁, h ▸ acc₂⟩
+
+theorem egraph_unique {pcr : PCR S} (h : pcr = graph.pcr) : graph ≍ pcr.egraph := by
+  sorry
+  -- TODO: We might not be able to prove this up to HEq, but only some weaker notion of
+  --       isomorphism.
+
+end PCR
