Eqsat/TreeAutomaton/Reachable.lean
@@ -1,0 +1,41 @@
+import Eqsat.TreeAutomaton.Basic
+
+namespace TreeAutomaton
+
+variable [Signature S] {auto : TreeAutomaton S Q}
+
+-- A given state is reachable (from a ground term) if:
+-- 1. it is the destination of a transition for a constant, or
+-- 2. it is the destination of a transition where all source states are reachable.
+inductive IsReachableState (auto : TreeAutomaton S Q) : Q → Prop where
+  | const (mem : tr ∈ auto.trans) : (Signature.arity tr.sym = 0) → IsReachableState auto tr.dst
+  | trans (mem : tr ∈ auto.trans) : (∀ i, IsReachableState auto <| tr.srcs i) → IsReachableState auto tr.dst
+
+-- The set of reachable states.
+abbrev ReachableState (auto : TreeAutomaton S Q) : Type :=
+  { q // auto.IsReachableState q }
+
+def IsReachableTransition (auto : TreeAutomaton S Q) (tr : Transition S Q) : Prop :=
+  ∀ i, auto.IsReachableState <| tr.srcs i
+
+def Transition.liftReachable {auto : TreeAutomaton S Q} (tr : Transition S auto.ReachableState) :
+    Transition S Q where
+  sym  := tr.sym
+  srcs := (tr.srcs ·)
+  dst  := tr.dst
+
+def reachableTrans (auto : TreeAutomaton S Q) : Set (Transition S auto.ReachableState) :=
+  { tr | auto.IsReachableTransition tr.liftReachable }
+
+def reachableFinal (auto : TreeAutomaton S Q) : Set auto.ReachableState :=
+  { q | ↑q ∈ auto.final ∧ auto.IsReachableState q }
+
+-- The reachable sub-automaton prunes all unreachable states and transitions.
+def reachable (auto : TreeAutomaton S Q) : TreeAutomaton S auto.ReachableState where
+  trans := auto.reachableTrans
+  final := auto.reachableFinal
+
+def reachable_preserves_confluence {auto : TreeAutomaton S Q} (con : auto.trs.Confluent) :
+    auto.reachable.trs.Confluent := by
+  intro t t₁ t₂ s₁ s₂
+  sorry
